narcissus: Improve readability of encoders (WIP)

src/Narcissus/Examples/README.v
@@ -205,19 +205,304 @@ Module Sensor5.
 
   Let encode := encoder_impl encoder_decoder.
 
+  (* Notation "x |> y" := (Projection_AlignedEncodeM y x _) (right associativity, at level 2). *)
   Goal Some (encoder_impl encoder_decoder) = None.
     unfold "|>".
 
-    Definition cmp {S sz cache} {cacheAdd: CacheAdd cache nat} (writer: AlignedEncodeM (S := S) sz) val :=
-      (fun (v0 : t Core.char sz) (idx : nat) (a: _) (env : CacheFormat) =>
-       writer v0 idx a env) val.
+    Definition Projection_AlignedEncodeM'
+               {S' S'' : Type}
+               {cache : Cache}
+               {sz}
+               (encode : AlignedEncodeM (S := S'') sz)
+               (f : S' -> S'')
+      : AlignedEncodeM (S := S') sz :=
+      fun v idx s' env =>
+        encode v idx (f s') env.
+
+    Lemma cleanup_aligned_encoder_init {cache S2}:
+      forall (sz : nat) (r : S2) (v : t Core.char sz) ch idx,
+      forall (f: @AlignedEncodeM cache _ sz)
+        (g: @AlignedEncodeM cache S2 sz)
+        (h: forall sz, S2 -> Vector.t Core.char sz -> _)
+        (h': @AlignedEncodeM cache S2 sz),
+        h' v idx r ch = h sz r v ->
+        (AppendAlignedEncodeM f g) v idx r ch = h' v idx r ch ->
+        (AppendAlignedEncodeM f g) v idx r ch = h sz r v.
+    Proof. intros; congruence. Qed.
+
+    Lemma cleanup_aligned_encoder_projection {cache S1 S2}:
+      forall (sz : nat) (r : S2) (v : t Core.char sz) ch idx,
+      forall (f: @AlignedEncodeM cache S1 sz)
+        (g: @AlignedEncodeM cache S2 sz)
+        proj x,
+        (AppendAlignedEncodeM
+           (Projection_AlignedEncodeM' f proj)
+           g) v idx r ch = x ->
+        (AppendAlignedEncodeM
+           (fun (v0 : t Core.char sz) (idx : nat) (s : S2) (env : CacheFormat) =>
+              f v0 idx (proj s) env)
+           g) v idx r ch = x.
+    Proof. compute; intros; congruence. Qed.
+
+    Lemma cleanup_aligned_encoder_bind {cache S2}:
+      forall (sz : nat) (r : S2) (v : t Core.char sz) ch idx,
+      forall (f g h: @AlignedEncodeM cache S2 sz),
+        (forall v idx r ch, g v idx r ch = h v idx r ch) ->
+        (AppendAlignedEncodeM f g) v idx r ch =
+        (AppendAlignedEncodeM f h) v idx r ch.
+    Proof. compute; intros; destruct (f _ _ _ _); congruence. Qed.
+
+    Lemma cleanup_aligned_encoder_assoc {cache S1 S2}:
+      forall (sz : nat) (r : S2) (v : t Core.char sz) ch idx,
+      forall (f1 f2: @AlignedEncodeM cache S1 sz)
+        (g: @AlignedEncodeM cache S2 sz)
+        proj x,
+        (AppendAlignedEncodeM
+           (fun (v0 : t Core.char sz) (idx : nat) (s : S2) (env : CacheFormat) =>
+              f1 v0 idx (proj s) env)
+           (AppendAlignedEncodeM
+              (fun (v0 : t Core.char sz) (idx : nat) (s : S2) (env : CacheFormat) =>
+                 f2 v0 idx (proj s) env)
+              g)) v idx r ch = x ->
+        (AppendAlignedEncodeM
+           (fun (v0 : t Core.char sz) (idx : nat) (s : S2) (env : CacheFormat) =>
+              (AppendAlignedEncodeM f1 f2) v0 idx (proj s) env)
+           g) v idx r ch = x.
+    Proof. compute; intros; destruct (f1 _ _ _ _); [ destruct (f2 _ _ _ _) | ]; congruence. Qed.
+
+    Ltac derive_clean_encoder :=
+      intros;
+      eapply cleanup_aligned_encoder_init; [ reflexivity | ];
+      repeat (intros; first [ eapply cleanup_aligned_encoder_assoc |
+                              eapply cleanup_aligned_encoder_projection;
+                              [ | eapply cleanup_aligned_encoder_bind ] ]);
+      reflexivity.
+
+    Notation "x |> y" := (Projection_AlignedEncodeM' y x) (right associativity, at level 2).
+
+    Ltac exact_computed t :=
+      let t' := (eval compute in t) in exact t'.
+
+    Definition const {A B} (a: A) := fun (_: B) => a.
+
+    Ltac cleanup_encoder enc :=
+      let nm := fresh in
+      pose enc as nm;
+      simpl in nm;
+      repeat change (fun x => ?h x) with h in nm;
+      repeat change (wzero ?sz) with (ltac:(let w0 := (eval compute in (wzero sz)) in exact w0)) in nm;
+      repeat ((change (@split1' (S ?sz1) ?sz2 (WS ?b ?w)) with
+                   (ltac:(exact_computed (@split1' (S sz1) sz2 (WS b w)))) in nm) ||
+              (change (@split2' (S ?sz1) ?sz2 (WS ?b ?w)) with
+                   (ltac:(exact_computed (@split2' (S sz1) sz2 (WS b w)))) in nm));
+      repeat change (fun (_: ?B) => ?cst) with (ltac:(let A := (type of cst) in exact (@const A B cst))) in nm.
 
     match goal with
-    | [  |- context C[(fun (v0 : t Core.char _) (idx : nat) (s' : sensor_msg) (env : CacheFormat) =>
-                        ?wrt _ _ v0 idx (@?f s') env)] ] =>
-      pose wrt; pose f;
-      let C' := context C[cmp wrt (f s')] in
-      change C'
+    | [  |- Some ?f = None ] => pose f
+    end.
+
+    (* unfold split1', split2' in nm; simpl in nm; *)
+    (* fold @split1' in nm; fold @split2' in nm. *)
+
+    (* unfold SetCurrentBytes; simpl. *)
+
+    unfold SetCurrentBytes.
+    (* match goal with *)
+    (* | [  |- Some ?f = None ] => *)
+    (*   let g := constr:( *)
+    (*             ltac:(eexists; derive_clean_encoder) *)
+    (*             : { g : (forall sz : nat, sensor_msg -> t Core.char sz -> option (t Core.char sz * nat * @CacheFormat _)) *)
+    (*                     & forall (sz : nat) (r : sensor_msg) (v : t Core.char sz), f sz r v = g sz r v }) in *)
+    (*   cleanup_encoder (projT1 g) *)
+    (* end. *)
+
+    Goal True.
+      pose (fun (sz : nat) (r : sensor_msg) (v : t Core.char sz) =>
+       ((fun (v0 : t Core.char sz) (idx : nat) (s' : sensor_msg) (env : CacheFormat) =>
+         SetCurrentByte v0 idx (stationID s') env)>>
+        (fun (v0 : t Core.char sz) (idx : nat) (_ : sensor_msg) => SetCurrentByte v0 idx (wzero 8))>>
+        (fun (v0 : t Core.char sz) (idx : nat) (_ : sensor_msg) (env : CacheFormat) =>
+         SetCurrentBytes (sz := 2) v0 idx WO~0~0~0~0~0~1~1~1~1~1~1~0~0~0~1~0 env)>>
+        (fun (v0 : t Core.char sz) (idx : nat) (s' : sensor_msg) (env : CacheFormat) =>
+         SetCurrentByte v0 idx (natToWord 8 (| measurements s' |)) env)>>
+        (fun (v0 : t Core.char sz) (idx : nat) (s' : sensor_msg) (env : CacheFormat) =>
+         AlignedEncodeList (fun n : nat => SetCurrentBytes (sz := 2)) sz v0 idx (measurements s') env))%AlignedEncodeM v 0 r
+         tt) as f.
+      assert { g : (forall sz : nat, sensor_msg -> t Core.char sz -> option (t Core.char sz * nat * @CacheFormat test_cache))
+                                    & forall (sz : nat) (r : sensor_msg) (v : t Core.char sz), f sz r v = g sz r v }.
+      eexists; intros.
+      eapply cleanup_aligned_encoder_init; [ reflexivity | ].
+      repeat (intros; first [ eapply cleanup_aligned_encoder_assoc |
+                              eapply cleanup_aligned_encoder_bind ]).
+      
+
+      unfold SetCurrentBytes.
+      repeat change (fun x => ?h x) with h.
+      change (fun (v : t Core.char ?sz) (idx : nat) (s' : ?T) => ?f v idx ?cst) with
+          (fun (v : t Core.char sz) (idx : nat) (s' : T) => f v idx ((const cst) s')).
+      change (fun (v : t Core.char ?sz) (idx : nat) (s' : _) => ?f v idx (?g s')) with
+          (Projection_AlignedEncodeM' (sz := sz) f g).
+      change (fun (v : t Core.char ?sz) (idx : nat) (s' : _) => ?f v idx (?g1 (?g2 s'))) with
+          (Projection_AlignedEncodeM' (Projection_AlignedEncodeM' f g1) g2).
+      change (fun (v : t Core.char ?sz) (idx : nat) (s' : _) => ?f v idx (?g1 (?g2 (?g3 s')))) with
+          (Projection_AlignedEncodeM' (sz := sz) (Projection_AlignedEncodeM' (Projection_AlignedEncodeM' f g1) g2) g3).
+      
+      apply cleanup_aligned_encoder_bind; intros.
+          (Projection_AlignedEncodeM' (sz := sz) f g).
+      change (fun (v : t Core.char ?sz) (idx : nat) (s' : sensor_msg) =>
+                ?f v idx (?g s') env) with
+          (Projection_AlignedEncodeM' (sz := sz) f g).
+      
+      (intros; first [ eapply cleanup_aligned_encoder_assoc |
+                       eapply cleanup_aligned_encoder_projection;
+                       eapply cleanup_aligned_encoder_bind ]).
+
+      (intros; first [ eapply cleanup_aligned_encoder_assoc
+                     |
+                     eapply cleanup_aligned_encoder_bind ]).
+      (intros; first [ eapply cleanup_aligned_encoder_assoc;
+                       [ | eapply cleanup_aligned_encoder_projection] |
+                       eapply cleanup_aligned_encoder_bind ]).
+      (intros; first [ eapply cleanup_aligned_encoder_assoc;
+                       [ | eapply cleanup_aligned_encoder_projection] |
+                       eapply cleanup_aligned_encoder_bind ]).
+      (intros; first [ eapply cleanup_aligned_encoder_assoc;
+                       [ | eapply cleanup_aligned_encoder_projection] |
+                       eapply cleanup_aligned_encoder_bind ]).
+      (intros; first [ eapply cleanup_aligned_encoder_assoc;
+                       [ | eapply cleanup_aligned_encoder_projection] |
+                       eapply cleanup_aligned_encoder_bind ]).
+      (intros; first [ eapply cleanup_aligned_encoder_assoc;
+                       [ | eapply cleanup_aligned_encoder_projection] |
+                       eapply cleanup_aligned_encoder_bind ]).
+      (intros; first [ eapply cleanup_aligned_encoder_assoc;
+                       [ | eapply cleanup_aligned_encoder_projection] |
+                       eapply cleanup_aligned_encoder_bind ]).
+      (intros; first [ eapply cleanup_aligned_encoder_assoc |
+                       eapply cleanup_aligned_encoder_projection |
+                       eapply cleanup_aligned_encoder_bind ]).
+      Focus 2.
+            (intros; first [ eapply cleanup_aligned_encoder_assoc |
+                       eapply cleanup_aligned_encoder_projection |
+                       eapply cleanup_aligned_encoder_bind ]).
+
+      unfold SetCurrentBytes.
+      (intros; first [ eapply cleanup_aligned_encoder_assoc |
+                       eapply cleanup_aligned_encoder_bind ]).
+      (intros; first [ eapply cleanup_aligned_encoder_assoc |
+                       eapply cleanup_aligned_encoder_bind ]).
+      (intros; first [ eapply cleanup_aligned_encoder_assoc |
+                       eapply cleanup_aligned_encoder_bind ]).
+      (intros; first [ eapply cleanup_aligned_encoder_assoc |
+                       eapply cleanup_aligned_encoder_bind ]).
+      (intros; first [ eapply cleanup_aligned_encoder_assoc |
+                       eapply cleanup_aligned_encoder_bind ]).
+      (intros; first [ eapply cleanup_aligned_encoder_assoc |
+                       eapply cleanup_aligned_encoder_bind ]).
+      (intros; first [ eapply cleanup_aligned_encoder_assoc |
+                       eapply cleanup_aligned_encoder_bind ]).
+      derive_clean_encoder.
+        intros;
+        [ reflexivity | ].
+      unfold SetCurrentBytes.
+      cleanup_encoder enc
+      intros;
+        first [eapply cleanup_aligned_encoder_bind |
+               eapply cleanup_aligned_encoder_bind_const ].
+      Show Proof.
+      intros.
+
+      repeat change (fun (v : Vector.t Core.char _) (idx : nat) (_ : ?tmsg) (env : @CacheFormat ?cache) =>
+                       ?f v idx ?x env)
+        with (fun (v : Vector.t Core.char _) (idx : nat) (s : tmsg) (env : @CacheFormat cache) =>
+                f v idx ((fun _ => x) s) env).
+
+      eapply cleanup_aligned_encoder_bind.
+      unfold SetCurrentBytes.
+      intros.
+
+      eapply cleanup_aligned_encoder_assoc.
+      eapply cleanup_aligned_encoder_bind.
+      intros.
+      eapply cleanup_aligned_encoder_assoc.
+      eapply cleanup_aligned_encoder_bind.
+      intros.
+      eapply cleanup_aligned_encoder_bind.
+      intros.
+      eapply cleanup_aligned_encoder_bind.
+
+      
+      Show Proof.
+      (* FIXME remove bind_const *)
+      
+
+      
+      simpl.
+        Show Proof.
+
+
+        
+        reflexivity.
+
+      Show Proof.
+
+    reflexivity.
+    
+    stationID -> SetCurrentByte;
+    (const w0) -> SetCurrentByte;
+    (const WO~0~0~0~0~0~1~1~1~1~1~1~0~0~0~1~0) -> SetCurrentBytes;
+    measurements . length . natToWord 8 -> setCurrentByte;
+    measurements . AlignedEncodeList SetCurrentBytes
+
+    
+    stationID |> (@SetCurrentByte test_cache test_cache_add_nat)
+
+    
+    unfold "|>".
+
+    Definition cmp {A S sz cache} {cacheAdd: CacheAdd cache nat} (writer: AlignedEncodeM (S := S) sz) (f: A -> _) :=
+      (fun (v0 : t Core.char sz) (idx : nat) (a: _) (env : CacheFormat) =>
+       writer v0 idx (f a) env).
+
+    Set Printing Implicit.
+    Locate ">>".
+    (* Unset Printing Notations. *)
+    match goal with
+    | [  |- Some ?f = None ] =>
+      assert { g : (forall sz : nat, sensor_msg -> t Core.char sz -> option (t Core.char sz * nat * @CacheFormat test_cache))
+                   & forall (sz : nat) (r : sensor_msg) (v : t Core.char sz), f sz r v = g sz r v }
+    end.
+    eexists.
+    intros.
+    Open Scope AlignedEncodeM.
+
+    Lemma 
+    
+    simpl.
+      let g :  :=
+          ltac:(unshelve econstructor) in
+      
+      change f with
+          (fun (sz : nat) (r : sensor_msg) (v : t Core.char sz) =>
+             ltac:(let body := (eval cbv beta in (f sz r v)) in
+                   match body with
+                   | context[@AppendAlignedEncodeM test_cache sensor_msg _ ?y _] =>
+                     let body := (change y with
+                         (fun (v0 : t Core.char sz) (idx : nat) (s' : sensor_msg) (env : @CacheFormat test_cache) =>
+                            ltac:(let ybody := (eval cbv beta in (y v0 idx s' env)) in
+                                  match body with
+                                  | ?f v0 idx (@?g s') env =>
+                                    exact (idtac (fun x => f v0 idx x env) (g s'))
+                                  end)) in body) in
+                     exact body
+                   end))
+    end.
+    match goal with
+    | [  |- context [(fun (v0 : t Core.char _) (idx : nat) (s' : sensor_msg) (env : CacheFormat) =>
+                       @?f v0 idx s' env)] ] => idtac
+                                                 (* pose wrt; pose f *)
+                                                 (* let C' := context C[cmp (wrt sz c) f] in *)
+                                                 (* change C' *)
     end.
     Notation "[[[ xyz ===> f ]]]" :=
       ().
